\documentclass[12pt]{article}
\usepackage{amsmath}

\begin{document}
\begin{tabular}{c|c|c}
$v$ & Ascent Rate & m/s\\
$F$ & Free Lift & N\\
$F_g$ & Gross Lift & N\\
$C_d$ & Drag Coefficient &\\
$\rho_a$ & Air Density & kg/m$^3$\\
$\rho_g$ & Gas Density & kg/m$^3$\\
$r$ & Launch Radius & m\\
$A$ & Launch Area & m$^2$\\
$V_L$ & Launch Volume & m$^3$\\
$m_p$ & Payload Mass & kg\\
$m_b$ & Balloon Mass & kg\\
$g$ & Gravitational Acceleration & m/s$^2$\\
\end{tabular}
\newpage
\begin{align}
v &=\sqrt{\frac{F}{\frac{1}{2}C_d\rho_aA}}\\
A &=\pi r^2\\
F &=F_g - (m_p + m_b)(g)\\
F_g &= (\rho_a - \rho_g) \times V_L\\
V_L &= \frac{4}{3}\pi r^3\\
F_g &= (\rho_a - \rho_g)(\frac{4}{3}\pi r^3)\\
F &= (\rho_a - \rho_g)(\frac{4}{3}\pi r^3) - (m_p + m_b)(g)\\
v &= \sqrt{\frac
{(\rho_a - \rho_g)(\frac{4}{3}\pi r^3) - (m_p + m_b)(g)}
{(\frac{1}{2}C_d\rho_a)(\pi r^2)}}\\
v^2(\frac{1}{2}C_d\rho_a\pi r^2) &= ((\rho_a - \rho_g)\frac{4}{3}\pi r^3) -
(m_p + m_b)(g)\\
&[(\rho_a - \rho_g)\frac{4}{3}\pi]r^3 - [\frac{1}{2}v^2C_d\rho_a\pi]r^2 -
[(m_p + m_b)g] = 0
\end{align}
yuck! a cubic!
\end{document}
